progress on tactics

Lampe/Lampe/Lens.lean
@@ -21,7 +21,7 @@ def Access.get (acc : Access (Tp.denote p) tp₁ tp₂) (s : Tp.denote p tp₁) 
 
 def Access.modify (acc : Access (Tp.denote p) tp₁ tp₂) (s : Tp.denote p tp₁) (v' : Tp.denote p tp₂) : Option $ Tp.denote p tp₁ := match acc with
 | .tuple mem => Builtin.replaceTuple' s mem v'
-| .array (n := n) idx => if h : idx.toNat < n.toNat then Builtin.replaceArray' s ⟨idx.toNat, h⟩ v' else none
+| .array (n := n) idx => if h : idx.toNat < n.toNat then s.set ⟨idx.toNat, h⟩ v' else none
 | .slice idx => if h : idx.toNat < s.length then Builtin.replaceSlice' s ⟨idx.toNat, h⟩ v' else none
 
 @[simp]
